Sim work (#101)
* pushing current simulator work

* more simulator work

* removing stream map

Simulator/CoqSim/Simulator.v
@@ -15,18 +15,15 @@ Variable Word : nat -> Type.
 Variable Vec : nat -> Type -> Type.
 Variable Map : Type -> Type.
 Variable M : Type -> Type.
+Variable Arr : Type -> Type.
 
 Context `{IsWord Word}.
 Context `{IsVector Vec}.
 Context `{StringMap Map}.
 Context `{IOMonad Word Vec M}.
+Context `{IsArray Word Vec M Arr}.
 
 Notation "'do' x <- y ; cont" := (bind y (fun x => cont)) (at level 20).
-
-(* Variable KindInfo : Map string FullKind 
-Hypothesis ActionGood: forall Write r k in a, KindInfo r = k /\ forall Read r k in a, KindInfo r = k
-Lemma: SimRegGood: (r, k) in SimReg -> KindInfo r = k
-Theorem: ActionSimRegGood: forall Write r k in a, (r, k') in SimReg -> k = k' *)
 
 Definition eval_K := eval_Kind Word Vec.
 
@@ -79,12 +76,12 @@ Fixpoint mkProd(ts : list Type) : Type :=
   end.
 
 Class Environment E := {
-  envPre  : E -> FileState (V := Vec) (W := Word) (M := Map) -> SimRegs -> string -> M E;
-  envPost : E -> FileState (V := Vec) (W := Word) (M := Map) -> SimRegs -> string -> M E
+  envPre  : E -> FileState (V := Vec) (W := Word) (M := Map) (Arr := Arr) -> SimRegs -> string -> M E;
+  envPost : E -> FileState (V := Vec) (W := Word) (M := Map) (Arr := Arr) -> SimRegs -> string -> M E
   }.
 
 Definition meth_sig{E}`{Environment E}(sig : Signature) : Type :=
-  eval_K (fst sig) -> FileState (V := Vec) (W := Word) (M := Map) -> SimRegs -> E -> M (E * (eval_K (snd sig))).
+  eval_K (fst sig) -> FileState (V := Vec) (W := Word) (M := Map) (Arr := Arr) -> SimRegs -> E -> M (E * (eval_K (snd sig))).
 
 Definition dec_sig{E}`{Environment E}(dec : string * Signature) : Type :=
   meth_sig (snd dec).
@@ -100,17 +97,17 @@ Fixpoint return_meth{E}`{Environment E}(meth : string)(sig : Signature)(meths : 
 Proof.
   assert (sig = snd dec).
   rewrite <- pf; auto.
-  rewrite H6.
+  rewrite H12.
   exact (fst fs).
 Defined.
 
 Definition reg_not_found{X} : string -> M X :=
   fun reg => error ("register " ++ reg ++ " not found.").
 
-Fixpoint eval_ActionT{k}{E}`{Environment E}(env : E)(state : @FileState Vec Word Map)(meths : list (string * Signature))(updates : Updates)(fupdates : FileUpdates)(a : ActionT eval_K k)(a_wf : WfActionT_new init_regs a)(fs : mkProd (List.map dec_sig meths)){struct a} : M (Updates * FileUpdates * eval_K k).
+Fixpoint eval_ActionT{k}{E}`{Environment E}(env : E)(state : @FileState Vec Word Map Arr)(meths : list (string * Signature))(updates : Updates)(fupdates : FileUpdates)(a : ActionT eval_K k)(a_wf : WfActionT_new init_regs a)(fs : mkProd (List.map dec_sig meths)){struct a} : M (Updates * FileUpdates * eval_K k).
   refine (match a return WfActionT_new init_regs a -> _ with
-  | MCall meth s e cont => fun pf => 
-       match rf_methcall state meth (existT _ (fst s) (eval_E e)) with
+  | MCall meth s e cont => fun pf => io_do x <- rf_methcall state meth (existT _ (fst s) (eval_E e));
+       match x with
       | Some (o, existT k v) => match Kind_dec k (snd s) with
                                 | left _ => _
                                 | right _ => error ("Type mismatch")
@@ -170,8 +167,8 @@ Proof.
            inversion G; auto.
         ** destruct pf.
            clear G.
-           rewrite <- H6, <- H7 in f.
-           exact (eval_ActionT _ _ _ env state meths updates fupdates (cont f) (H8 _) fs).
+           rewrite <- H12, <- H13 in f.
+           exact (eval_ActionT _ _ _ env state meths updates fupdates (cont f) (H14 _) fs).
       * destruct pf.
    + exact (reg_not_found r).
   (* WriteReg *)
@@ -234,201 +231,10 @@ End Regs.
 
 Section Regs2.
 
-(* Definition consistent(regs1 regs2 : SimRegs) := forall r k,
-  (exists v, lookup String.eqb r regs1 = Some (existT _ k v)) <-> (exists v', lookup String.eqb r regs2 = Some (existT _ k v')).
-
-Lemma consistent_refl : forall regs, consistent regs regs.
-Proof.
-  intros regs r k; tauto.
-Qed.
-
-Lemma consistent_sym : forall regs1 regs2, consistent regs1 regs2 -> consistent regs2 regs1.
-Proof.
-  unfold consistent.
-  intros.
-  split; intro; apply H5; auto.
-Qed.
-
-Lemma consistent_trans : forall regs1 regs2 regs3, consistent regs1 regs2 -> consistent regs2 regs3 -> consistent regs1 regs3.
-Proof.
-  unfold consistent.
-  intros.
-  split; intro.
-  - apply H6; apply H5; auto.
-  - apply H5; apply H6; auto.
-Qed.
-
-Lemma lookup_cons : forall K V (eqb : K -> K -> bool) k k' v (ps : list (K*V)), lookup eqb k ((k',v)::ps) =
-  if eqb k k' then Some v else lookup eqb k ps.
-Proof.
-  intros.
-  unfold lookup.
-  unfold find.
-  simpl.
-  destruct (eqb k k'); auto.
-Qed.
-
-Lemma consistent_cons_cong : forall (regs1 regs2 : SimRegs)(r : SimReg), consistent regs1 regs2 -> consistent (r::regs1) (r::regs2).
-Proof.
-  unfold consistent.
-  intros regs regs2 r.
-  destruct r.
-  split.
-  - repeat rewrite lookup_cons.
-    destruct String.eqb.
-    + auto.
-    + apply H5.
-  - repeat rewrite lookup_cons.
-    destruct String.eqb.
-    + auto.
-    + apply H5.
-Qed.
-
-Lemma consistent_lemma : forall {k v r regs1 regs2}, consistent regs1 regs2 -> lookup String.eqb r regs1 = Some (existT _ k v) ->
-  exists v', lookup String.eqb r regs2 = Some (existT _ k v').
-Proof.
-  intros.
-  apply H5.
-  exists v; auto.
-Qed.
-
-Lemma wf_consistent_stable : forall {k} (a : ActionT eval_K k) init_regs regs1 regs2, consistent regs1 regs2 -> WfActionT_new init_regs a -> WfActionT_new init_regs a.
-Proof.
-  intros.
-  induction a; simpl.
-  - intro.
-    apply H7.
-    apply H6.
-  - intro.
-    apply H7.
-    apply H6.
-  - split.
-    + apply IHa.
-      apply H6.
-    + intro.
-      apply H7.
-      apply H6.
-  - intro.
-    apply H7.
-    apply H6.
-  - destruct lookup eqn:G.
-    + destruct s; split.
-      * simpl in H6.
-        destruct lookup eqn:G1 in H6.
-        ** destruct s.
-           rewrite G1 in G.
-           inversion G.
-           destruct H6.
-           congruence.
-        ** destruct H6.
-      * intro.
-        apply H7.
-        simpl in H6.
-        destruct lookup in H6.
-        ** destruct s; destruct H6.
-           apply H8.
-        ** destruct H6.
-   + simpl in H6.
-     destruct lookup eqn:G1.
-     * inversion G.
-     * auto.
-  - destruct lookup eqn:G.
-    + simpl in H6.
-      destruct lookup eqn:G1.
-      * destruct s.
-        split; destruct s0.
-        ** inversion G.
-           destruct H6.
-           congruence.
-        ** apply IHa; tauto.
-      * destruct H6.
-    + simpl in H6.
-      destruct lookup eqn:G1.
-      * destruct s.
-        inversion G.
-      * auto.
-  - simpl in H6.
-    repeat split.
-    + apply IHa1; tauto.
-    + apply IHa2; tauto.
-    + intro; apply H7.
-      apply H6.
-  - apply IHa.
-    exact H6.
-  - exact I.
-Qed.
-
-Lemma update_consistent : forall regs1 regs2 (upd : Update regs2), consistent regs1 regs2 -> consistent regs1 (do_single_update upd regs1).
-Proof.
-  intros.
-  split; intros [v Hv].
-  - pose (lookup_match upd).
-    destruct (r =? (reg_name upd)) eqn:G.
-    + rewrite String.eqb_eq in G.
-      rewrite G.
-      rewrite (@update_hit _ _ k v).
-      * rewrite <- G in e.
-        destruct (consistent_lemma H5 Hv) as [v' Hv'].
-        rewrite Hv' in e.
-        inversion e.
-        rewrite H7.
-        eexists; auto.
-      * rewrite <- G; auto.
-   + eexists.
-     rewrite String.eqb_neq in G.
-     rewrite update_miss; auto.
-     exact Hv.
-  - pose (lookup_match upd).
-    destruct (r =? (reg_name upd)) eqn:G.
-    + rewrite String.eqb_eq in G.
-      rewrite G in Hv.
-      assert (consistent regs2 regs1). apply consistent_sym; auto.
-      destruct (consistent_lemma H6 e) as [v' Hv'].
-      rewrite (@update_hit _ _ (kind upd) v') in Hv.
-      * rewrite <- G in e.
-        inversion Hv.
-        exists v'. rewrite G. exact Hv'.
-      * auto.
-   + eexists.
-     rewrite String.eqb_neq in G.
-     rewrite update_miss in Hv; auto.
-     exact Hv.
-Qed.
-
-Lemma updates_consistent : forall (regs : SimRegs)(upds : Updates regs), consistent regs (do_updates upds regs).
-Proof.
-  intros; induction upds; simpl.
-  - apply consistent_refl.
-  - apply (@consistent_trans _ (do_updates upds regs)).
-    * auto.
-    * apply update_consistent.
-      apply consistent_sym.
-      auto.
-Qed. *)
-
-(* Lemma wf_updates_stable{k} : forall (regs : SimRegs)(upds : Updates regs)(a : ActionT eval_K k),
-  WfActionT_new regs a -> WfActionT_new (do_updates upds regs) a.
-Proof.
-  intros.
-  apply (@wf_consistent_stable _ _ regs).
-  - apply updates_consistent.
-  - auto.
-Qed. *)
-
-(*
-Definition maintain_wf{k} regs (upds : Updates regs) (a : ActionT eval_K k) : {r : RuleT & wf_action regs a} -> {r : RuleT & wf_action (do_updates upds regs) a}.
-Proof.
-   intros [r w].
-   exists r.
-   apply wf_updates_stable.
-   exact w.
-Defined.
-*)
-
 Lemma update_hit : forall init_regs regs k v (upd : Update init_regs), lookup String.eqb (reg_name upd) regs = Some (existT _ k v) -> lookup String.eqb (reg_name upd) (do_single_update upd regs) = Some (existT _ (kind upd) (new_val upd)).
 Proof.
   induction regs; intros.
-  - discriminate H5.
+  - discriminate H11.
   - simpl do_single_update.
     destruct a.
     destruct String.eqb eqn:G.
@@ -438,9 +244,9 @@ Proof.
     + rewrite lookup_cons.
       rewrite G.
       eapply IHregs.
-      rewrite lookup_cons in H5.
-      rewrite G in H5.
-      exact H5.
+      rewrite lookup_cons in H11.
+      rewrite G in H11.
+      exact H11.
 Qed.
 
 Lemma update_miss : forall r init_regs regs (upd : Update init_regs), r <> reg_name upd -> lookup String.eqb r (do_single_update upd regs) = lookup String.eqb r regs.
@@ -452,9 +258,9 @@ Proof.
     destruct String.eqb eqn:G.
     + repeat rewrite lookup_cons.
       rewrite String.eqb_eq in G.
-      rewrite G in H5.
-      rewrite <- String.eqb_neq in H5.
-      rewrite H5.
+      rewrite G in H11.
+      rewrite <- String.eqb_neq in H11.
+      rewrite H11.
       auto.
     + repeat rewrite lookup_cons.
       destruct (r =? s).
@@ -465,21 +271,21 @@ Qed.
 Lemma lookup_update : forall init_regs regs k x (upd : Update init_regs) r, lookup String.eqb r (do_single_update upd regs) = Some (existT (fun x : FullKind => fullType eval_K x) k x) -> exists k' y, lookup String.eqb r regs = Some (existT _ k' y).
 Proof.
   induction regs; intros.
-  - discriminate H5.
-  - simpl do_single_update in H5.
+  - discriminate H11.
+  - simpl do_single_update in H11.
     destruct a.
     destruct (reg_name upd =? s).
-    + rewrite lookup_cons in H5.
+    + rewrite lookup_cons in H11.
       rewrite lookup_cons.
       destruct (r =? s).
       * destruct s0; repeat eexists; reflexivity.
-      * repeat eexists; exact H5.
-    + rewrite lookup_cons in H5.
+      * repeat eexists; exact H11.
+    + rewrite lookup_cons in H11.
       rewrite lookup_cons.
       destruct (r =? s).
       * destruct s0; repeat eexists; reflexivity.
       * eapply IHregs.
-        exact H5.
+        exact H11.
 Qed.
 
 Lemma update_consistent : forall (curr_regs : SimRegs)(init_regs : list RegInitT)(upd : Update init_regs),
@@ -490,46 +296,46 @@ Proof.
   - destruct (String.eqb r (reg_name upd)) eqn:G.
     + rewrite String.eqb_eq in G.
       rewrite G.
-      destruct (kc_init_sim kc _ H5).
+      destruct (kc_init_sim kc _ H11).
       erewrite update_hit.
       * pose (lookup_match upd) as lk.
         rewrite <- G in lk.
-        rewrite H5 in lk.
+        rewrite H11 in lk.
         inversion lk.
-        rewrite H8 in *.
+        rewrite H14 in *.
         eexists; auto.
       * rewrite <- G.
-        destruct (kc_init_sim kc _ H5).
-        exact H6.
+        destruct (kc_init_sim kc _ H11).
+        exact H12.
     + rewrite String.eqb_neq in G.
       erewrite update_miss; auto.
       apply kc.
-      eexists; exact H5.
+      eexists; exact H11.
   - destruct (String.eqb r (reg_name upd)) eqn:G.
     + rewrite String.eqb_eq in G.
-      rewrite G in H5.
-      destruct (lookup_update _ _ _ H5) as [k' [y Hy]].
-      erewrite update_hit in H5.
+      rewrite G in H11.
+      destruct (lookup_update _ _ _ H11) as [k' [y Hy]].
+      erewrite update_hit in H11.
       * pose (lookup_match upd) as lk.
         rewrite G.
-        inversion H5.
+        inversion H11.
         eexists; exact lk.
       * exact Hy.
     + rewrite String.eqb_neq in G.
-      erewrite update_miss in H5; auto.
-      destruct (kc_sim_init kc _ H5).
-      eexists; exact H6.
+      erewrite update_miss in H11; auto.
+      destruct (kc_sim_init kc _ H11).
+      eexists; exact H12.
 Qed.
 
 Lemma updates_consistent : forall (init_regs : list RegInitT)(curr_regs : SimRegs)(upds : list (Update init_regs)),
   kind_consistent init_regs curr_regs -> kind_consistent init_regs (do_updates upds curr_regs).
 Proof.
   induction upds; intro.
-  - exact H5.
+  - exact H11.
   - apply update_consistent; auto.
 Qed.
 
-Fixpoint eval_Rules{E}`{Environment E}(env : E)(state : FileState (V := Vec) (W := Word) (M := Map))(numRules : nat)(meths : list (string * Signature))(init_regs : list (string * {x : FullKind & RegInitValT x}))(curr_regs : SimRegs)(kc_curr : kind_consistent init_regs curr_regs)(rules : Stream {r : RuleT & WfActionT_new init_regs (snd r eval_K)}){struct numRules} : mkProd (List.map dec_sig meths) -> M unit. refine
+Fixpoint eval_Rules{E}`{Environment E}(env : E)(state : FileState (V := Vec) (W := Word) (M := Map) (Arr := Arr))(numRules : nat)(meths : list (string * Signature))(init_regs : list (string * {x : FullKind & RegInitValT x}))(curr_regs : SimRegs)(kc_curr : kind_consistent init_regs curr_regs)(rules : Stream {r : RuleT & WfActionT_new init_regs (snd r eval_K)}){struct numRules} : mkProd (List.map dec_sig meths) -> M unit. refine
   match numRules with
   | 0 => fun fs => error "TIMEOUT"
   | S numRules' => fun fs => match rules with
@@ -537,16 +343,14 @@ Fixpoint eval_Rules{E}`{Environment E}(env : E)(state : FileState (V := Vec) (W 
                                 do env' <- envPre env state curr_regs (fst (projT1 r));
                                 do p <- eval_RuleT _ env' state meths (projT1 r) (projT2 r)  fs;
                                 do env'' <- envPost env' state curr_regs (fst (projT1 r));
-                                eval_Rules _ _  env'' (exec_file_updates state (snd (fst p))) numRules' meths init_regs (do_updates (fst (fst p)) curr_regs) _ (Streams.map _ rules') fs
+                                do state' <- exec_file_updates state (snd (fst p));
+                                eval_Rules _ _  env'' state' numRules' meths init_regs (do_updates (fst (fst p)) curr_regs) _ (rules') fs
                                 )
                             end
   end.
 Proof.
   - exact kc_curr.
   - apply updates_consistent; auto.
-  - intros [rule wf].
-    exists rule.
-    exact wf.
 Defined.
 
 Definition initialize_SimRegs(regs : list RegInitT) : SimRegs :=
@@ -567,8 +371,8 @@ Proof.
   intros.
   induction rules.
   - exact [].
-  - simpl in H5; destruct H5.
-    exact ((existT _ a H5) :: (IHrules H6)).
+  - simpl in H11; destruct H11.
+    exact ((existT _ a H11) :: (IHrules H12)).
 Defined.
 
 Lemma kc_nil : kind_consistent [] [].
@@ -579,13 +383,13 @@ Qed.
 Lemma kc_cons : forall init_regs regs r k v v', kind_consistent init_regs regs -> kind_consistent ((r,(existT _ k v)) :: init_regs) ((r, (existT _ k v')) :: regs).
 Proof.
   intros.
-  intros r' k'; split; intro; rewrite lookup_cons in *; destruct (r' =? r) eqn:G; destruct H6.
-  - inversion H6.
+  intros r' k'; split; intro; rewrite lookup_cons in *; destruct (r' =? r) eqn:G; destruct H12.
+  - inversion H12.
     eexists; auto.
-  - apply (kc_init_sim H5 _ H6).
-  - inversion H6.
+  - apply (kc_init_sim H11 _ H12).
+  - inversion H12.
     eexists; auto.
-  - apply (kc_sim_init H5 _ H6).
+  - apply (kc_sim_init H11 _ H12).
 Qed.
 
 Lemma init_regs_kc : forall init_regs, kind_consistent init_regs (initialize_SimRegs init_regs).
@@ -612,10 +416,10 @@ Proof.
   - unfold WfBaseModule_new in pf.
     destruct pf.
     refine (do state <- initialize_files args rfbs;
-    eval_Rules env state (timeout * (List.length rules)) meths _ (unwind_list (get_wf_rules _ _ (H6 _)) _) fs).
+    eval_Rules env state (timeout * (List.length rules)) meths _ (unwind_list (get_wf_rules _ _ (H12 _)) _) fs).
     + apply init_regs_kc.
     + simpl.
-      destruct H6; discriminate.
+      destruct H12; discriminate.
 Defined.
 
 Definition eval_BaseMod{E}`{Environment E}(env : E)(args : list (string * string))(rfbs : list RegFileBase)(timeout : nat)(meths : list (string * Signature))(basemod : BaseModule)(wf : WfBaseModule_new basemod) :=
@@ -625,7 +429,7 @@ End Regs2.
 
 End EvalAction.
 
-Definition eval_BaseMod_Haskell := @eval_BaseMod HWord HVec HMap IO _ _ _ _.
+Definition eval_BaseMod_Haskell := @eval_BaseMod HWord HVec HMap IO HArray _ _ _ _.
 
 Section Eval_Wf.
 
@@ -633,13 +437,16 @@ Variable Word : nat -> Type.
 Variable Vec : nat -> Type -> Type.
 Variable Map : Type -> Type.
 Variable M : Type -> Type.
+Variable Arr : Type -> Type.
 
 Context `{IsWord Word}.
 Context `{IsVector Vec}.
 Context `{StringMap Map}.
 Context `{IOMonad Word Vec M}.
+Context `{IsArray Word Vec IO Arr}.
 
-Definition eval_BaseMod_Wf{E}`{Environment _ _ _ _ E}(env : E)(args : list (string * string))(rfbs : list RegFileBase)(timeout : nat)(meths : list (string * Signature))(basemod : BaseModule)(wf : WfBaseModule basemod) :=
+Definition eval_BaseMod_Wf{E}`{Environment _ _ _ _ _ E}(env : E)(args : list (string * string))(rfbs : list RegFileBase)(timeout : nat)(meths : list (string * Signature))(basemod : BaseModule)(wf : WfBaseModule basemod) :=
   curry _ (eval_Basemodule_rr env args rfbs timeout meths (WfBaseModule_WfBaseModule_new wf)).
+
 
 End Eval_Wf.
